made fairmerge a bit better

src/demo/fairmerge/FMAutomat.thy
@@ -6,26 +6,34 @@ begin
 
 setup_lifting type_definition_ndAutomaton
 
-(*FM automaton*)
-fun dAfm_transition::"S_fm \<Rightarrow> (bool\<times> bool) \<Rightarrow> (S_fm \<times> bool)set"where
-"dAfm_transition (S True 0 [] buf2) (bool1,bool2) = {((S (False) next [] (buf2@[bool2])),(bool1)) | next. True} "|
-"dAfm_transition (S False 0 buf1 []) (bool1,bool2) = {((S (True) next (buf1@[bool1]) []),(bool2)) | next. True} "|
-"dAfm_transition (S True 0 buf1 buf2) (bool1,bool2) = {((S (False) next ((tl buf1)@[bool1]) (buf2@[bool2])),(hd buf1)) | next. True} "|
-"dAfm_transition (S False 0 buf1 buf2) (bool1,bool2) = {((S (True) next (buf1@[bool1]) ((tl buf2)@[bool2])),(hd buf2)) | next. True} "|
-"dAfm_transition (S True n [] buf2) (bool1,bool2) = {((S (True) (n-1)  [] (buf2@[bool2])),(bool1))}"|
-"dAfm_transition (S False n buf1 []) (bool1,bool2) = {((S (False) (n-1) (buf1@[bool1]) []),(bool2))}"|
-"dAfm_transition (S True n buf1 buf2) (bool1,bool2) = {((S (True) (n-1) ((tl buf1)@[bool1]) (buf2@[bool2])),(hd buf1))}"|
-"dAfm_transition (S False n buf1 buf2) (bool1,bool2) = {((S (False) (n-1) ((buf1)@[bool1]) ((tl buf2)@[bool2])),(hd buf2))}"
+fun dAfm_case::"bool \<Rightarrow> nat \<Rightarrow> nat list \<Rightarrow> nat list \<Rightarrow> (nat\<times> nat) \<Rightarrow> (S_fm \<times> nat)"where
+"dAfm_case True  n [] l2 (nat1,nat2) = (S True  n []          (l2@[nat2]), nat1)"|
+"dAfm_case False n l1 [] (nat1,nat2) = (S False n (l1@[nat1]) []         , nat2)"|
 
-definition fairmergetransition::"(S_fm \<Rightarrow> inFM\<^sup>\<surd> \<Rightarrow> ((S_fm \<times> outFM\<^sup>\<surd>) set))"where
+"dAfm_case True  n (nhd#l1) l2       (nat1,nat2) = (S True  n (l1@[nat1]) (l2@[nat2]),nhd)"|
+"dAfm_case False n l1       (nhd#l2) (nat1,nat2) = (S False n (l1@[nat1]) (l2@[nat2]),nhd)"
+
+(*FM automaton*)
+fun dAfm_transition::"S_fm \<Rightarrow> (nat\<times> nat) \<Rightarrow> (S_fm \<times> nat)set"where
+"dAfm_transition (S bool 0       buf1 buf2) input = {dAfm_case (\<not>bool) n buf1 buf2 input | n. True} "|
+"dAfm_transition (S bool (Suc n) buf1 buf2) input = {dAfm_case bool    n buf1 buf2 input}"
+
+definition fairmergetransition::"(S_fm \<Rightarrow> inFM\<^sup>\<surd> \<Rightarrow> ((S_fm \<times> outFM\<^sup>\<Omega>) set))"where
 "fairmergetransition state insbe = ( let Set = (dAfm_transition state (fmInSBE.getter(insbe))) in
-                                   (\<lambda>e. (fst e, fmOutSBE.setter(snd e)))` Set)"
+                                   (\<lambda>e. (fst e, fmOutSB.setter(\<up>(snd e))))` Set)"
 
 definition fairmergeinit::"(S_fm \<times> outFM\<^sup>\<Omega>) set" where
 "fairmergeinit = {(S bool n [] [], \<bottom>) | bool n. True}"
 
-lift_definition FairMerge::"(S_fm,inFM,outFM) ndAutomaton" is
-"(undefined, fairmergeinit)" (*fairmergetransition works with sbElem instead of sb*)
-  sorry
+definition FairMerge::"(S_fm,inFM,outFM) ndAutomaton_incomplete" where
+"FairMerge = (|ndaiTransition = fairmergetransition, ndaiInitConfig = fairmergeinit|)"
+
+lift_definition FairMergelift::"(S_fm,inFM,outFM) ndAutomaton" is
+"(fairmergetransition, fairmergeinit)"
+  apply auto
+  apply(simp add: fairmergetransition_def)
+  apply(case_tac state;case_tac x1;case_tac x2;case_tac x3;case_tac x4,auto)
+  apply (metis (mono_tags)old.prod.exhaust)+
+  by(simp add: fairmergeinit_def,auto)
 
 end
